\subsection{}

Let~$α$ be a natural isomorphism from~$H_A$ to~$H_{A'}$.
This means that we have for every set~$B$ a bijection
\[
	α_B \colon \cat{A}(B, A) \to \cat{A}(B, A') \,,
\]
and these bijections are compatible in the sense that for every morphism
\[
	g \colon B \to B'
\]
in~$\cat{B}$, the following square diagram commutes:
\begin{equation}
	\label{naturality diagram for proving that yoneda reflects isomorphisms}
	\begin{tikzcd}[sep = large]
		\cat{A}(B', A)
		\arrow{r}[above]{α_B}
		\arrow{d}[left]{g^*}
		&
		\cat{A}(B', A')
		\arrow{d}[right]{g^*}
		\\
		\cat{A}(B, A)
		\arrow{r}[above]{α_{B'}}
		&
		\cat{A}(B, A')
	\end{tikzcd}
\end{equation}
Under the bijection
\[
	α_A \colon \cat{A}(A, A) \to \cat{A}(A, A') \,,
\]
the identity morphism of~$A$ has an image in~$\cat{A}(A, A')$, which we will denote by~$φ$.
Similarly, under the bijection
\[
	α_{A'} \colon \cat{A}(A', A) \to \cat{A}(A, A) \,,
\]
the identity morphism of~$A'$ has a unique preimage in~$\cat{A}(A', A)$, which we will denote by~$ψ$.

We have thus found two morphisms
\[
	φ \colon A \to A' \,,
	\quad
	ψ \colon A' \to A \,.
\]
We consider now the commutative diagram~\eqref{naturality diagram for proving that yoneda reflects isomorphisms} in the special cases of~$φ$ and~$ψ$ in place of~$g$, i.e., the following two commutative diagrams:
\[
	\begin{tikzcd}[sep = large]
		\cat{A}(A', A)
		\arrow{r}[above]{α_A}
		\arrow{d}[left]{φ^*}
		&
		\cat{A}(A', A')
		\arrow{d}[right]{φ^*}
		\\
		\cat{A}(A, A)
		\arrow{r}[above]{α_{A'}}
		&
		\cat{A}(A, A')
	\end{tikzcd}
	\qquad
	\begin{tikzcd}[sep = large]
		\cat{A}(A, A)
		\arrow{r}[above]{α_A}
		\arrow{d}[left]{ψ^*}
		&
		\cat{A}(A, A')
		\arrow{d}[right]{ψ^*}
		\\
		\cat{A}(A', A)
		\arrow{r}[above]{α_{A'}}
		&
		\cat{A}(A', A')
	\end{tikzcd}
\]
We get from the commutativity of the left-hand diagram that
\[
	α_{A'}( ψ ∘ φ )
	=
	α_{A'}( φ^*(ψ) )
	=
	φ^*( α_A(ψ) )
	=
	φ^*( \id_{A'} )
	=
	\id_{A'} ∘ φ
	=
	φ
	=
	α_{A'}( \id_A ) \,,
\]
and therefore
\[
	ψ ∘ φ = \id_A
\]
by the injectivity of~$α_{A'}$.
We also get from the commutativity of the right-hand diagram that
\[
	φ ∘ ψ
	=
	ψ^*( φ )
	=
	ψ^*( α_A( \id_A) )
	=
	α_{A'}( ψ )
	=
	\id_{A'} \,.
\]
These calculations show that the two morphisms~$φ$ and~$ψ$ are mutually inverse, and therefore in particular that~$A$ and~$A'$ are isomorphic.
