\subsection{}





\subsubsection{}

If~$g$ is a morphism from~$B$ to~$B'$ in~$\Bcat$ then the pair~$(\id_A, g)$ is a morphism from~$(A, B)$ to~$(A, B')$ in~$\Acat \times \Bcat$.
It follows that~$F(\id_A, g)$ is a morphism from~$F(A, B) = F^A(B)$ to~$F(A, B') = F^A(B')$ in~$\Ccat$.
We have
\[
	F^A(\id_B)
	=
	F(\id_A, \id_B)
	=
	F( \id_{(A, B)} )
	=
	\id_{F(A, B)}
	=
	\id_{F^A(B)}
\]
for ever object~$B$ of~$\Bcat$.
For every three objects~$B$,~$B'$,~$B''$ of~$\Bcat$ and every two composable morphisms~$g$ from~$B$ to~$B'$ and~$g'$ from~$B'$ to~$B''$ in~$\Bcat$ we have
\begin{align*}
	F^A(g') \circ F^A(g)
	&=
	F(\id_A, g') \circ F(\id_A, g)
	\\
	&=
	F( (\id_A, g') \circ (\id_A, g) )
	\\
	&=
	F(\id_A \circ \id_A, g' \circ g)
	\\
	&=
	F(\id_A, g' \circ g)
	\\
	&=
	F^A(g' \circ g) \,.
\end{align*}
This shows that~$F^A$ is indeed a functor from~$\Bcat$ to~$\Ccat$.

Let now~$B$ be a fixed object of the category~$\Bcat$.
For every object~$A$ of~$\Acat$ let~$F_B(A)$ be the object~$F(A, B)$ of~$\Acat \times \Bcat$, and for every morphism~$f$ from~$A$ to~$A'$ in~$\Acat$ let~$F_B(f)$ be the morphism~$F(f, \id_B)$ from~$(A, B) = F_B(A)$ to~$(A', B) = F_{B'}(A)$ in~$\Ccat$.

We have
\[
	F_B(\id_A)
	=
	F(\id_A, \id_B)
	=
	F( \id_{(A, B)} )
	=
	\id_{F(A, B)}
	=
	\id_{F_B(A)}
\]
for every object~$A$ of~$\Acat$.
For every three objects~$A$,~$A'$,~$A''$ of~$\Acat$ and every two morphisms~$f$ from~$A$ to~$A'$ and~$f'$ from~$A'$ to~$A''$ in~$\Acat$ we have
\begin{align*}
	F_B(f') \circ F_B(f)
	&=
	F(f', \id_B) \circ F(f, \id_B)
	\\
	&=
	F( (f', \id_B) \circ (f, \id_B) )
	\\
	&=
	F( f' \circ f, \id_B \circ \id_B )
	\\
	&=
	F( f' \circ f, \id_B )
	\\
	&=
	F_B( f' \circ f ) \,.
\end{align*}
This shows that~$F_B$ is indeed a functor.





\subsubsection{}

We have
\[
	F^A(B)
	=
	(A, B)
	=
	F_B(A)
\]
for every object~$A$ of~$\Acat$ and every object~$B$ of~$\Bcat$.
We also have
\begin{align*}
	F^{A'}(g) \circ F_B(f)
	&=
	F(\id_{A'}, g) \circ F(f, \id_B)
	\\
	&=
	F( (\id_{A'}, g) \circ (f, \id_B) )
	\\
	&=
	F(f, g)
	\\
	&=
	F( (f, \id_{B'}) \circ (\id_A, g) )
	\\
	&=
	F(f, \id_{B'}) \circ F(\id_A, g)
	\\
	&=
	F_{B'}(f) \circ F^A(g)
\end{align*}
for every two object~$A$ and~$A'$ in~$\Acat$, every two objects~$B$ and~$B'$ in~$\Bcat$, and every two morphisms~$f$ from~$A$ to~$A'$ in~$\Acat$ and~$g$ from~$B$ to~$B'$ in~$\Bcat$.





\subsubsection{}

Suppose first that such a fuctor~$F$ were to exist.
Then
\[
	F(A, B)
	=
	F^A(B)
\]
for every object~$(A, B)$ of~$\Acat \times \Bcat$, and
\[
	F(f, g)
	=
	F( (\id_{A'}, g) \circ (f, \id_B) )
	=
	F(\id_{A'}, g) \circ F(f, \id_B)
	=
	F^{A'}(g) \circ F_B(f)
\]
for every morphism~$(f, g)$ from~$(A, B)$ to~$(A', B')$ in~$\Acat \times \Bcat$.

This shows the uniqueness of~$F$.
We will now show the existence of~$F$.

For every object~$A$ of~$\Acat$ and~$B$ of~$\Bcat$ let we denote the element~$F^A(B)$ by~$F(A, B)$.
We have equivalently~$F(A B) = F_B(A)$.

Let~$f$ be a morphism from~$A$ to~$A'$ in~$\Acat$ and let~$g$ be a morphism from~$B$ to~$B'$ in~$\Bcat$.
We denote the morphism~$F^{A'}(g) \circ F_B(f)$ in~$\Ccat$ by~$F(f, g)$.
We have equivalently~$F(f, g) = F_{B'}(f) \circ F^{A}(g)$.
The morphism~$F_B(f)$ goes from~$F_B(A) = F(A, B)$ to~$F_B(A') = F(A', B)$, and the morphism~$F^{A'}(g)$ goes from~$F^{A'}(B) = F(A', B)$ to~$F^{A'}(B') = F(A', B')$.
It follows that the morphism~$F(f, g)$ goes from~$F(A, B)$ to~$F(A', B')$.

The assignment~$F$ satisfies
\begin{align*}
	F( \id_{(A, B)} )
	&=
	F( \id_A, \id_B )
	\\
	&=
	F^A(\id_B) \circ F_B(\id_A)
	\\
	&=
	\id_{F^A(B)} \circ \id_{F_B(A)}
	\\
	&=
	\id_{F(A, B)} \circ \id_{F(A, B)}
	\\
	&=
	\id_{F(A, B)} \,.
\end{align*}
For every three objects~$(A, B)$,~$(A', B')$,~$(A'', B'')$ of~$\Acat \times \Bcat$ and every two morphisms~$(f, g)$ from~$(A, B)$ and~$(f', g')$ from~$(A', B')$ to~$(A'', B'')$ in~$\Acat \times \Bcat$ we have
\begin{align*}
	F(f', g') \circ F(f, g)
	&=
	F^{A''}(g') \circ F_{B'}(f') \circ F_{B'}(f) \circ F^A(g)
	\\
	&=
	F^{A''}(g') \circ F_{B'}(f' \circ f) \circ F^A(g)
	\\
	&=
	F^{A''}(g') \circ F^{A''}(g) \circ F_B(f' \circ f)
	\\
	&=
	F^{A''}(g' \circ g) \circ F_B(f' \circ f)
	\\
	&=
	F(g' \circ g, f' \circ f)
	\\
	&=
	F( (g', f') \circ (g, f) )
	\\
	&=
	F(g', f') \circ F(g, f) \,.
\end{align*}
This shows altogether that the assignment~$F$ is indeed a functor.




