\subsection{}

Let~$F$ be a functor from~$\cat{A}$ to~$\cat{B}$.
We can regard~$F$ as a functor from~$\cat{A}^{\op}$ to~$\cat{B}^{\op}$, which we shall denote by~$F'$ instead of~$F$ for clarity.
This functor~$F'$ is given by
\[
	F'( A^{\op} ) = F(A)^{\op}
	\quad\text{and}\quad
	F'( f^{\op} ) = F(f)^{\op}
\]
for every object~$A$ of~$\cat{A}$ and every morphism~$f$ in~$\cat{A}$.
This assignment~$F'$ is indeed a functor from~$\cat{A}^{\op}$ to~$\cat{B}^{\op}$:
\begin{itemize}

	\item
		We have for every object~$A$ of~$\cat{A}$ the equalities
		\[
			F'( \id_{A^{\op}} )
			=
			F'( \id_A^{\op} )
			=
			F(\id_A)^{\op}
			=
			\id_{F(A)}^{\op}
			=
			\id_{F(A)^{\op}} \,.
		\]

	\item
		We have for every two composable morphisms
		\[
			f \colon A \to A' \,,
			\quad
			g \colon A' \to A''
		\]
		in~$\cat{A}$ the equalities
		\begin{align*}
			\SwapAboveDisplaySkip
			F'( f^{\op} g^{\op} )
			&=
			F'( (gf)^{\op} )
			\\
			&=
			F(gf)^{\op}
			\\
			&=
			( F(g) F(f) )^{\op}
			\\
			&=
			F(f)^{\op} F(g)^{\op}
			\\
			&=
			F'(f^{\op}) F'(g^{\op}) \,.
		\end{align*}

\end{itemize}
This shows that~$F'$ is indeed a functor from~$\cat{A}^{\op}$ to~$\cat{B}^{\op}$.
We have therefore the map
\begin{equation}
	\label{opposite_on_objects}
	(\ph)'
	\colon
	\Ob([\cat{A}, \cat{B}])
	\to
	\Ob([\cat{A}^{\op}, \cat{B}^{\op}]) \,.
\end{equation}

Let~$F$ and~$G$ be two functors from~$\cat{A}$ to~$\cat{B}$ and let~$α$ be a natural transformation from~$F$ to~$G$.
We have for every morphism
\[
	f \colon A \to A'
\]
in~$\cat{A}$ the following commutative square diagram in~$\cat{B}$:
\[
	\begin{tikzcd}[sep = large]
		F(A)
		\arrow{r}[above]{F(f)}
		\arrow{d}[left]{α_A}
		&
		F(A')
		\arrow{d}[right]{α_{A'}}
		\\
		G(A)
		\arrow{r}[above]{G(f)}
		&
		G(A')
	\end{tikzcd}
\]
It follows that we have the following commutative diagram in~$\cat{B}^{\op}$:
\[
	\begin{tikzcd}[row sep = large, column sep = huge]
		F(A)^{\op}
		&
		F(A')^{\op}
		\arrow{l}[above]{F(f)^{\op}}
		\\
		G(A)^{\op}
		\arrow{u}[left]{α_A^{\op}}
		&
		G(A')^{\op}
		\arrow{u}[right]{α_{A'}^{\op}}
		\arrow{l}[above]{G(f)^{\op}}
	\end{tikzcd}
\]
This diagram can also be written as follows:
\[
	\begin{tikzcd}[row sep = large, column sep = huge]
		F'(A^{\op})
		&
		F'(A'^{\op})
		\arrow{l}[above]{F'(f^{\op})}
		\\
		G'(A^{\op})
		\arrow{u}[left]{α_A^{\op}}
		&
		G'(A'^{\op})
		\arrow{u}[right]{α_{A'}^{\op}}
		\arrow{l}[above]{G'(f^{\op})}
	\end{tikzcd}
\]
The commutativity of the above diagram shows we have a natural transformation~$α'$ from~$G'$ to~$F'$ with components~$(α')_{A^{\op}} ≔ α_A^{\op}$ for every object~$A$ of~$\cat{A}$.

The natural transformation~$α'$ depends contravariantly functorial on~$α$:
\begin{itemize}

	\item
		Let~$F$ be a functor from~$\cat{A}$ from~$\cat{B}$.
		We have the chain of equalities
		\[
			( \id_F' )_{A^{\op}}
			=
			\id_F(A)^{\op}
			=
			\id_{F(A)}^{\op}
			=
			\id_{F(A)^{\op}}
			=
			\id_{F'(A^{\op})}
			=
			\id_{F'}(A^{\op})
		\]
		for every object~$A$ of~$\cat{A}$.
		This shows that~$\id_F' = \id_{F'}$.

	\item
		Let~$F$,~$G$ and~$H$ be functors from~$\cat{A}$ to~$\cat{B}$, and let
		\[
			α \colon F \To G \,,
			\quad
			β \colon G \To H
		\]
		be natural transformations.
		We have the induces natural transformation
		\[
			α' \colon G' \To F' \,,
			\quad
			β' \colon H' \To G' \,,
			\quad
			(β α)' \colon H' \To F' \,.
		\]
		We have for every object~$A$ of~$\cat{A}$ the chain of equalities
		\[
			(α' β')_{A^{\op}}
			=
			(α')_{A^{\op}} (β')_{A^{\op}}
			=
			α_A^{\op} β_A^{\op}
			=
			(β_A α_A)^{\op}
			=
			(β α)_A^{\op}
			=
			( (β α)' )_{A^{\op}} \,,
		\]
		and therefore altogether the equality
		\[
			α' β' = (β α)' \,.
		\]

\end{itemize}



We have altogether shown that the mapping~\eqref{opposite_on_objects} extends to a contravariant functor
\[
	D_{\cat{A}, \cat{B}}
	\colon
	[\cat{A}, \cat{B}]
	\to
	[\cat{A}^{\op}, \cat{B}^{\op}] \,,
\]
We claim that the two contravariant functors~$D_{\cat{A}, \cat{B}}$ and~$D_{\cat{A}^{\op}, \cat{B}^{\op}}$ are mutually inverse.
This then shows that~$D_{\cat{A}, \cat{B}}$ is an isomorphism of categories from~$[\cat{A}, \cat{B}]^{\op}$ to~$[\cat{A}^{\op}, \cat{B}^{\op}]$.

Indeed, we have
\[
	D_{\cat{A}^{\op}, \cat{B}^{\op}}( D_{\cat{A}, \cat{B}}( F ) )
	=
	D_{\cat{A}^{\op}, \cat{B}^{\op}}( F' )
	=
	F''
	=
	F
\]
for every object~$F$ of~$[\cat{A}, \cat{B}]$, and similarly
\[
	D_{\cat{A}^{\op}, \cat{B}^{\op}}( D_{\cat{A}, \cat{B}}( α ) )
	=
	D_{\cat{A}^{\op}, \cat{B}^{\op}}( α' )
	=
	α''
	=
	α
\]
for every morphism~$α$ in~$[\cat{A}, \cat{B}]$.
These equalities show that the composite~$D_{\cat{A}^{\op}, \cat{B}^{\op}} ∘ D_{\cat{A}, \cat{B}}$ is the identity functor of~$[\cat{A}, \cat{B}]$.
It follows that also
\[
	D_{\cat{A}, \cat{B}} ∘ D_{\cat{A}^{\op}, \cat{B}^{\op}}
	=
	D_{\cat{A}^{\op\op}, \cat{B}^{\op\op}} ∘ D_{\cat{A}^{\op}, \cat{B}^{\op}}
	=
	\Id_{[\cat{A}^{\op}, \cat{B}^{\op}]} \,.
\]
