\subsection{}

Suppose first that condition~(a) is satisfied.
The relations~$a ≤ g(f(a))$ and~$f(g(b)) ≤ b$ from condition~(b) are then equivalent to the relations~$f(a) ≤ f(a)$ and~$g(b) ≤ g(b)$, which hold true.
We hence find that condition~(b) follows from condition~(a).

If on the other hand condition~(b) is satisfied, then it follows that
\[
	f(a) ≤ b
	\implies
	g(f(a)) ≤ g(b)
	\implies
	a ≤ g(b)
\]
and
\[
	a ≤ g(b)
	\implies
	f(a) ≤ f(g(b))
	\implies
	f(a) ≤ b
\]
for any two elements~$a$ of~$A$ and~$b$ of~$B$.
We hence find that condition~(a) follows from condition~(b).
